src/lib/data/Kuiper.Tensor.fst
@@ -20,7 +20,7 @@ inline_for_extraction noextract
 let from_array
   (#et : Type0) (#r : erased nat) (#d : idesc r)
   (l : tlayout d)
-  (a : larray et (tlayout_size l))
+  (a : larray et (tlayout_ulen l))
   : tensor et l
   = A.from_array (tensor_aview et l) a
 
@@ -29,7 +29,7 @@ let core
   (#et : Type0) (#r : erased nat) (#d : idesc r)
   (#l : tlayout d)
   (a : tensor et l)
-  : larray et (tlayout_size l)
+  : larray et (tlayout_ulen l)
   = A.core a
 
 let lem_core_from_array
@@ -43,7 +43,7 @@ let lem_core_from_array
 let lem_from_array_core
   (#et : Type0) (#r : nat) (#d : idesc r)
   (#l : tlayout d)
-  (p : larray et (tlayout_size l))
+  (p : larray et (tlayout_ulen l))
   : Lemma (ensures core (from_array l p) == p)
           [SMTPat (from_array l p)]
   = ()
@@ -126,7 +126,7 @@ fn tensor_pts_to_ref
   preserves
     a |-> Frac f s
   ensures
-    pure (SZ.fits (tlayout_size l))
+    pure (SZ.fits (tlayout_ulen l))
 {
   unfold tensor_pts_to a #f s;
   A.varray_pts_to_ref a;
@@ -143,11 +143,11 @@ fn tensor_pts_to_ref_located
   preserves
     on loc (a |-> Frac f s)
   ensures
-    pure (SZ.fits (tlayout_size l))
+    pure (SZ.fits (tlayout_ulen l))
 {
   map_loc loc
     #(a |-> Frac f s)
-    #(a |-> Frac f s ** pure (SZ.fits (tlayout_size l)))
+    #(a |-> Frac f s ** pure (SZ.fits (tlayout_ulen l)))
   fn _ {
     tensor_pts_to_ref a;
   };
@@ -199,7 +199,7 @@ fn tensor_abs
   (#et:Type)
   (#r : nat) (#d : idesc r)
   (l : tlayout d { is_full l })
-  (p : larray et (tlayout_size l))
+  (p : larray et (tlayout_ulen l))
   (#f : perm)
   (#s : chest d et)
   requires
@@ -221,9 +221,9 @@ fn tensor_abs'
   (#et:Type)
   (#r : nat) (#d : idesc r)
   (l : tlayout d { is_full l })
-  (p : larray et (tlayout_size l))
+  (p : larray et (tlayout_ulen l))
   (#f : perm)
-  (#s : lseq et (tlayout_size l))
+  (#s : lseq et (tlayout_ulen l))
   requires
     p |-> Frac f s
   ensures
@@ -371,7 +371,7 @@ fn tensor_implode
   (#f : perm)
   (#s : chest d et)
   requires
-    pure (SZ.fits (tlayout_size l))
+    pure (SZ.fits (tlayout_ulen l))
   requires
     forall+ (i : abs d).
       Cell a i |-> Frac f (acc s i)
@@ -398,7 +398,7 @@ fn tensor_ilower
   requires
     a |-> Frac f s
   ensures
-    pure (SZ.fits (tlayout_size l)) **
+    pure (SZ.fits (tlayout_ulen l)) **
     (forall+ (i : abs d).
       pts_to_cell (core a) #f (l.imap.f i) (acc s i))
 {
@@ -424,7 +424,7 @@ fn tensor_iraise
   (#f : perm)
   (#s : chest d et)
   requires
-    pure (SZ.fits (tlayout_size l)) **
+    pure (SZ.fits (tlayout_ulen l)) **
     (forall+ (i : abs d).
       pts_to_cell (core a) #f (l.imap.f i) (acc s i))
   ensures
